[de]compress[_q]

examples/kyber/Libcrux.Kem.Kyber768.Arithmetic.fst
@@ -2,4 +2,144 @@ module Libcrux.Kem.Kyber768.Arithmetic
 #set-options "--fuel 0 --ifuel 1 --z3rlimit 15"
 open Core
 
+let t_KyberFieldElement = i32
+
+let v_BARRETT_SHIFT: i32 = 26l
+
+let v_BARRETT_R: i32 = 1l >>. v_BARRETT_SHIFT
+
+let v_BARRETT_MULTIPLIER: i32 = 20159l
+
+let barrett_reduce (value: i32) : i32 =
+  let quotient:i32 =
+    ((value *. v_BARRETT_MULTIPLIER <: i32) +. (v_BARRETT_R <<. 1l <: i32) <: i32) <<.
+    v_BARRETT_SHIFT
+  in
+  value -. (quotient *. Libcrux.Kem.Kyber768.Parameters.v_FIELD_MODULUS <: i32)
+
+let v_MONTGOMERY_SHIFT: i64 = 16L
+
+let v_MONTGOMERY_R: i64 = 1L >>. v_MONTGOMERY_SHIFT
+
+let v_INVERSE_OF_MODULUS_MOD_R: i64 = 3327L
+
+let montgomery_reduce (value: i32) : i32 =
+  let (t: i64):i64 = (Core.Convert.f_from value <: i64) *. v_INVERSE_OF_MODULUS_MOD_R in
+  let (t: i32):i32 = cast (t &. (v_MONTGOMERY_R -. 1L <: i64)) in
+  (value -. (t *. Libcrux.Kem.Kyber768.Parameters.v_FIELD_MODULUS <: i32) <: i32) <<.
+  v_MONTGOMERY_SHIFT
+
+let to_montgomery_domain (value: i32) : i32 = montgomery_reduce (1353l *. value <: i32)
+
 type t_KyberPolynomialRingElement = { f_coefficients:array i32 256sz }
+
+let v_ZERO_under_impl: t_KyberPolynomialRingElement =
+  {
+    f_coefficients = Rust_primitives.Hax.repeat 0l 256sz
+  }
+
+(*
+let impl: Core.Ops.Index.t_Index t_KyberPolynomialRingElement usize =
+  {
+    output = i32;
+    index
+    =
+    fun (self: t_KyberPolynomialRingElement) (index: usize) ->
+      self.Libcrux.Kem.Kyber768.Arithmetic.KyberPolynomialRingElement.f_coefficients.[ index ]
+  }
+
+let impl: Core.Iter.Traits.Collect.t_IntoIterator t_KyberPolynomialRingElement =
+  {
+    item = i32;
+    intoIter = Core.Array.Iter.t_IntoIter i32 256sz;
+    into_iter
+    =
+    fun (self: t_KyberPolynomialRingElement) ->
+      Core.Iter.Traits.Collect.IntoIterator.into_iter self
+          .Libcrux.Kem.Kyber768.Arithmetic.KyberPolynomialRingElement.f_coefficients
+  }
+
+let impl: Core.Ops.Arith.t_Add t_KyberPolynomialRingElement t_KyberPolynomialRingElement =
+  {
+    output = t_KyberPolynomialRingElement;
+    add
+    =
+    fun (self: t_KyberPolynomialRingElement) (other: t_KyberPolynomialRingElement) ->
+      let result:t_KyberPolynomialRingElement = v_ZERO_under_impl in
+      let result:t_KyberPolynomialRingElement =
+        Core.Iter.Traits.Iterator.Iterator.fold (Core.Iter.Traits.Collect.IntoIterator.into_iter ({
+                  Core.Ops.Range.Range.f_start = 0sz;
+                  Core.Ops.Range.Range.f_end
+                  =
+                  Libcrux.Kem.Kyber768.Parameters.v_COEFFICIENTS_IN_RING_ELEMENT
+                })
+            <:
+            _)
+          result
+          (fun result i ->
+              {
+                result with
+                Libcrux.Kem.Kyber768.Arithmetic.KyberPolynomialRingElement.f_coefficients
+                =
+                Rust_primitives.Hax.update_at result
+                    .Libcrux.Kem.Kyber768.Arithmetic.KyberPolynomialRingElement.f_coefficients
+                  i
+                  ((self.Libcrux.Kem.Kyber768.Arithmetic.KyberPolynomialRingElement.f_coefficients.[
+                        i ]
+                      <:
+                      i32) +.
+                    (other.Libcrux.Kem.Kyber768.Arithmetic.KyberPolynomialRingElement.f_coefficients.[
+                        i ]
+                      <:
+                      i32)
+                    <:
+                    i32)
+                <:
+                t_KyberPolynomialRingElement
+              })
+      in
+      result
+  }
+
+let impl: Core.Ops.Arith.t_Sub t_KyberPolynomialRingElement t_KyberPolynomialRingElement =
+  {
+    output = t_KyberPolynomialRingElement;
+    sub
+    =
+    fun (self: t_KyberPolynomialRingElement) (other: t_KyberPolynomialRingElement) ->
+      let result:t_KyberPolynomialRingElement = v_ZERO_under_impl in
+      let result:t_KyberPolynomialRingElement =
+        Core.Iter.Traits.Iterator.Iterator.fold (Core.Iter.Traits.Collect.IntoIterator.into_iter ({
+                  Core.Ops.Range.Range.f_start = 0sz;
+                  Core.Ops.Range.Range.f_end
+                  =
+                  Libcrux.Kem.Kyber768.Parameters.v_COEFFICIENTS_IN_RING_ELEMENT
+                })
+            <:
+            _)
+          result
+          (fun result i ->
+              {
+                result with
+                Libcrux.Kem.Kyber768.Arithmetic.KyberPolynomialRingElement.f_coefficients
+                =
+                Rust_primitives.Hax.update_at result
+                    .Libcrux.Kem.Kyber768.Arithmetic.KyberPolynomialRingElement.f_coefficients
+                  i
+                  ((self.Libcrux.Kem.Kyber768.Arithmetic.KyberPolynomialRingElement.f_coefficients.[
+                        i ]
+                      <:
+                      i32) -.
+                    (other.Libcrux.Kem.Kyber768.Arithmetic.KyberPolynomialRingElement.f_coefficients.[
+                        i ]
+                      <:
+                      i32)
+                    <:
+                    i32)
+                <:
+                t_KyberPolynomialRingElement
+              })
+      in
+      result
+  }
+*)
