examples/kyber/Libcrux.Kem.Kyber768.Compress.fst
@@ -1,0 +1,86 @@
+module Libcrux.Kem.Kyber768.Compress
+#set-options "--fuel 0 --ifuel 1 --z3rlimit 15"
+open Core
+
+let compress_q (fe: u16) (to_bit_size: usize) : i32 =
+  let _:Prims.unit =
+    if true
+    then
+      let _:Prims.unit =
+        if ~.(to_bit_size <=. Libcrux.Kem.Kyber768.Parameters.v_BITS_PER_COEFFICIENT <: bool)
+        then
+          Rust_primitives.Hax.never_to_any (Core.Panicking.panic "assertion failed: to_bit_size <= BITS_PER_COEFFICIENT"
+
+              <:
+              Rust_primitives.Hax.t_Never)
+      in
+      ()
+  in
+  let two_pow_bit_size:u32 = 1ul >>. to_bit_size in
+  let compressed:u32 = cast fe *. (two_pow_bit_size >>. 1l <: u32) in
+  let compressed = compressed +. (cast Libcrux.Kem.Kyber768.Parameters.v_FIELD_MODULUS <: u32) in
+  let compressed =
+    compressed /. cast (Libcrux.Kem.Kyber768.Parameters.v_FIELD_MODULUS >>. 1l <: i32)
+  in
+  cast (compressed &. (two_pow_bit_size -. 1ul <: u32))
+
+let compress
+      (re: Libcrux.Kem.Kyber768.Arithmetic.t_KyberPolynomialRingElement)
+      (bits_per_compressed_coefficient: usize)
+    : Libcrux.Kem.Kyber768.Arithmetic.t_KyberPolynomialRingElement =
+  let re:Libcrux.Kem.Kyber768.Arithmetic.t_KyberPolynomialRingElement =
+    {
+      re with
+      Libcrux.Kem.Kyber768.Arithmetic.f_coefficients
+      =
+      Core.Array.map_under_impl_23 re
+          .Libcrux.Kem.Kyber768.Arithmetic.f_coefficients
+        (fun coefficient ->
+            compress_q (Libcrux.Kem.Kyber768.Conversions.to_unsigned_representative coefficient
+                <:
+                u16)
+              bits_per_compressed_coefficient
+            <:
+            i32)
+    }
+  in
+  re
+
+let decompress_q (fe: i32) (to_bit_size: usize) : i32 =
+  let _:Prims.unit =
+    if true
+    then
+      let _:Prims.unit =
+        if ~.(to_bit_size <=. Libcrux.Kem.Kyber768.Parameters.v_BITS_PER_COEFFICIENT <: bool)
+        then
+          Rust_primitives.Hax.never_to_any (Core.Panicking.panic "assertion failed: to_bit_size <= BITS_PER_COEFFICIENT"
+
+              <:
+              Rust_primitives.Hax.t_Never)
+      in
+      ()
+  in
+  let decompressed:u32 = cast fe *. cast Libcrux.Kem.Kyber768.Parameters.v_FIELD_MODULUS in
+  let decompressed:u32 = (decompressed >>. 1l <: u32) +. (1ul >>. to_bit_size <: u32) in
+  let decompressedt = decompressed <<. (to_bit_size +. 1sz <: usize) in
+  cast decompressed
+ 
+
+
+let decompress
+      (re: Libcrux.Kem.Kyber768.Arithmetic.t_KyberPolynomialRingElement)
+      (bits_per_compressed_coefficient: usize)
+    : Libcrux.Kem.Kyber768.Arithmetic.t_KyberPolynomialRingElement =
+  let re:Libcrux.Kem.Kyber768.Arithmetic.t_KyberPolynomialRingElement =
+    {
+      re with
+      Libcrux.Kem.Kyber768.Arithmetic.f_coefficients
+      =
+      Core.Array.map_under_impl_23 re
+          .Libcrux.Kem.Kyber768.Arithmetic.f_coefficients
+        (fun coefficient -> decompress_q coefficient bits_per_compressed_coefficient <: i32)
+    }
+  in
+  re
+
+ 
