examples/kyber/Libcrux.Kem.Kyber768.Constant_time_ops.fst
@@ -1,0 +1,118 @@
+module Libcrux.Kem.Kyber768.Constant_time_ops
+#set-options "--fuel 0 --ifuel 1 --z3rlimit 15"
+open Core
+
+let is_non_zero (value: u8) : u8 =
+  let value_negated:i8 = Core.Ops.Arith.Neg.neg (cast value) in
+  ((value |. cast value_negated <: u8) <<. 7l <: u8) &. 1uy
+
+let compare_ciphertexts_in_constant_time (lhs rhs: slice u8) : u8 =
+  let _:Prims.unit =
+    if true
+    then
+      let _:Prims.unit =
+        match Core.Slice.len_under_impl lhs, Core.Slice.len_under_impl rhs with
+        | left_val, right_val ->
+          if ~.(left_val =. right_val <: bool)
+          then
+            let kind:Core.Panicking.t_AssertKind = Core.Panicking.AssertKind_Eq in
+            Rust_primitives.Hax.never_to_any (Core.Panicking.assert_failed kind
+                  left_val
+                  right_val
+                  Core.Option.Option_None
+                <:
+                Rust_primitives.Hax.t_Never)
+      in
+      ()
+  in
+  let _:Prims.unit =
+    if true
+    then
+      let _:Prims.unit =
+        match Core.Slice.len_under_impl lhs, Libcrux.Kem.Kyber768.v_CIPHERTEXT_SIZE with
+        | left_val, right_val ->
+          if ~.(left_val =. right_val <: bool)
+          then
+            let kind:Core.Panicking.t_AssertKind = Core.Panicking.AssertKind_Eq in
+            Rust_primitives.Hax.never_to_any (Core.Panicking.assert_failed kind
+                  left_val
+                  right_val
+                  Core.Option.Option_None
+                <:
+                Rust_primitives.Hax.t_Never)
+      in
+      ()
+  in
+  let (r: u8):u8 = 0uy in
+  let r:Prims.unit =
+    Core.Iter.Traits.Iterator.Iterator.fold (Core.Iter.Traits.Collect.IntoIterator.into_iter ({
+              Core.Ops.Range.Range.f_start = 0sz;
+              Core.Ops.Range.Range.f_end = Libcrux.Kem.Kyber768.v_CIPHERTEXT_SIZE
+            })
+        <:
+        _)
+      r
+      (fun r i -> r |. ((lhs.[ i ] <: u8) ^. (rhs.[ i ] <: u8) <: u8) <: Prims.unit)
+  in
+  is_non_zero r
+
+let select_shared_secret_in_constant_time (lhs rhs: slice u8) (selector: u8) : array u8 32sz =
+  let _:Prims.unit =
+    if true
+    then
+      let _:Prims.unit =
+        match Core.Slice.len_under_impl lhs, Core.Slice.len_under_impl rhs with
+        | left_val, right_val ->
+          if ~.(left_val =. right_val <: bool)
+          then
+            let kind:Core.Panicking.t_AssertKind = Core.Panicking.AssertKind_Eq in
+            Rust_primitives.Hax.never_to_any (Core.Panicking.assert_failed kind
+                  left_val
+                  right_val
+                  Core.Option.Option_None
+                <:
+                Rust_primitives.Hax.t_Never)
+      in
+      ()
+  in
+  let _:Prims.unit =
+    if true
+    then
+      let _:Prims.unit =
+        match Core.Slice.len_under_impl lhs, Libcrux.Kem.Kyber768.v_SHARED_SECRET_SIZE with
+        | left_val, right_val ->
+          if ~.(left_val =. right_val <: bool)
+          then
+            let kind:Core.Panicking.t_AssertKind = Core.Panicking.AssertKind_Eq in
+            Rust_primitives.Hax.never_to_any (Core.Panicking.assert_failed kind
+                  left_val
+                  right_val
+                  Core.Option.Option_None
+                <:
+                Rust_primitives.Hax.t_Never)
+      in
+      ()
+  in
+  let mask:u8 = Core.Num.wrapping_sub_under_impl_6 (is_non_zero selector <: u8) 1uy in
+  let out:array u8 32sz = Rust_primitives.Hax.repeat 0uy 32sz in
+  let out:array u8 32sz =
+    Core.Iter.Traits.Iterator.Iterator.fold (Core.Iter.Traits.Collect.IntoIterator.into_iter ({
+              Core.Ops.Range.Range.f_start = 0sz;
+              Core.Ops.Range.Range.f_end = Libcrux.Kem.Kyber768.v_SHARED_SECRET_SIZE
+            })
+        <:
+        _)
+      out
+      (fun out i ->
+          Rust_primitives.Hax.update_at out
+            i
+            ((out.[ i ] <: u8) |.
+              (((lhs.[ i ] <: u8) &. mask <: u8) |. ((rhs.[ i ] <: u8) &. (~.mask <: u8) <: u8)
+                <:
+                u8)
+              <:
+              Prims.unit)
+          <:
+          array u8 32sz)
+  in
+  out
