examples/kyber/Libcrux.Kem.Kyber768.Conversions.fst
@@ -1,0 +1,116 @@
+module Libcrux.Kem.Kyber768.Conversions
+#set-options "--fuel 0 --ifuel 1 --z3rlimit 15"
+open Core
+
+(*
+let into_padded_array (#len: usize) (slice: slice u8) : array u8 v_LEN =
+  let _:Prims.unit =
+    if true
+    then
+      let _:Prims.unit =
+        if ~.((Core.Slice.len_under_impl slice <: usize) <=. v_LEN <: bool)
+        then
+          Rust_primitives.Hax.never_to_any (Core.Panicking.panic "assertion failed: slice.len() <= LEN"
+
+              <:
+              Rust_primitives.Hax.t_Never)
+      in
+      ()
+  in
+  let out:array u8 v_LEN = Rust_primitives.Hax.repeat 0uy v_LEN in
+  let out:array u8 v_LEN =
+    Rust_primitives.Hax.update_at out
+      ({
+          Core.Ops.Range.Range.f_start = 0sz;
+          Core.Ops.Range.Range.f_end = Core.Slice.len_under_impl slice <: usize
+        })
+      (Core.Slice.copy_from_slice_under_impl (Core.Ops.Index.IndexMut.index_mut out
+              ({
+                  Core.Ops.Range.Range.f_start = 0sz;
+                  Core.Ops.Range.Range.f_end = Core.Slice.len_under_impl slice <: usize
+                })
+            <:
+            slice u8)
+          slice
+        <:
+        slice u8)
+  in
+  out
+
+class t_UpdatingArray (v_Self: Type) = { push:self -> slice u8 -> self }
+
+type t_UpdatableArray = {
+  f_value:array u8 v_LEN;
+  f_pointer:usize
+}
+
+let new_under_impl (#len: usize) (value: array u8 v_LEN) : t_UpdatableArray v_LEN =
+  {
+    Libcrux.Kem.Kyber768.Conversions.UpdatableArray.f_value = value;
+    Libcrux.Kem.Kyber768.Conversions.UpdatableArray.f_pointer = 0sz
+  }
+
+let array_under_impl (#len: usize) (self: t_UpdatableArray v_LEN) : array u8 v_LEN =
+  self.Libcrux.Kem.Kyber768.Conversions.UpdatableArray.f_value
+
+let impl (#len: usize) : t_UpdatingArray (t_UpdatableArray v_LEN) =
+  {
+    push
+    =
+    fun (#len: usize) (self: t_UpdatableArray v_LEN) (other: slice u8) ->
+      let self:t_UpdatableArray v_LEN =
+        {
+          self with
+          Libcrux.Kem.Kyber768.Conversions.UpdatableArray.f_value
+          =
+          Rust_primitives.Hax.update_at (Libcrux.Kem.Kyber768.Conversions.UpdatableArray.f_value self
+
+              <:
+              t_UpdatableArray v_LEN)
+            ({
+                Core.Ops.Range.Range.f_start
+                =
+                self.Libcrux.Kem.Kyber768.Conversions.UpdatableArray.f_pointer;
+                Core.Ops.Range.Range.f_end
+                =
+                self.Libcrux.Kem.Kyber768.Conversions.UpdatableArray.f_pointer +.
+                (Core.Slice.len_under_impl other <: usize)
+                <:
+                usize
+              })
+            (Core.Slice.copy_from_slice_under_impl (Core.Ops.Index.IndexMut.index_mut self
+                      .Libcrux.Kem.Kyber768.Conversions.UpdatableArray.f_value
+                    ({
+                        Core.Ops.Range.Range.f_start
+                        =
+                        self.Libcrux.Kem.Kyber768.Conversions.UpdatableArray.f_pointer;
+                        Core.Ops.Range.Range.f_end
+                        =
+                        self.Libcrux.Kem.Kyber768.Conversions.UpdatableArray.f_pointer +.
+                        (Core.Slice.len_under_impl other <: usize)
+                        <:
+                        usize
+                      })
+                  <:
+                  slice u8)
+                other
+              <:
+              slice u8)
+        }
+      in
+      let self:t_UpdatableArray v_LEN =
+        {
+          self with
+          Libcrux.Kem.Kyber768.Conversions.UpdatableArray.f_pointer
+          =
+          self.Libcrux.Kem.Kyber768.Conversions.UpdatableArray.f_pointer +.
+          (Core.Slice.len_under_impl other <: usize)
+        }
+      in
+      self
+  }
+
+  *)
+  
+let to_unsigned_representative (fe: i32) : u16 =
+  cast (fe +. ((fe <<. 15l <: i32) &. Libcrux.Kem.Kyber768.Parameters.v_FIELD_MODULUS <: i32))
