examples/kyber/Libcrux.Kem.Kyber768.Ind_cpa.fst
@@ -1,0 +1,689 @@
+module Libcrux.Kem.Kyber768.Ind_cpa
+#set-options "--fuel 0 --ifuel 1 --z3rlimit 15"
+open Core
+
+let t_CiphertextCpa = array u8 1088sz
+
+type t_KeyPair = {
+  f_sk:array u8 1152sz;
+  f_pk:array u8 1184sz
+}
+
+let new_under_impl (sk: array u8 1152sz) (pk: array u8 1184sz) : t_KeyPair =
+  { Libcrux.Kem.Kyber768.Ind_cpa.KeyPair.f_sk = sk; Libcrux.Kem.Kyber768.Ind_cpa.KeyPair.f_pk = pk }
+
+let serialize_secret_key_under_impl (self: t_KeyPair) (implicit_rejection_value: slice u8)
+    : array u8 2400sz =
+  Libcrux.Kem.Kyber768.Conversions.array_under_impl (Libcrux.Kem.Kyber768.Conversions.UpdatingArray.push
+        (Libcrux.Kem.Kyber768.Conversions.UpdatingArray.push (Libcrux.Kem.Kyber768.Conversions.UpdatingArray.push
+                (Libcrux.Kem.Kyber768.Conversions.UpdatingArray.push (Libcrux.Kem.Kyber768.Conversions.new_under_impl
+                        (Rust_primitives.Hax.repeat 0uy 2400sz <: array u8 2400sz)
+                      <:
+                      Libcrux.Kem.Kyber768.Conversions.t_UpdatableArray 2400sz)
+                    (Rust_primitives.unsize self.Libcrux.Kem.Kyber768.Ind_cpa.KeyPair.f_sk
+                      <:
+                      slice u8)
+                  <:
+                  Libcrux.Kem.Kyber768.Conversions.t_UpdatableArray 2400sz)
+                (Rust_primitives.unsize self.Libcrux.Kem.Kyber768.Ind_cpa.KeyPair.f_pk <: slice u8)
+              <:
+              Libcrux.Kem.Kyber768.Conversions.t_UpdatableArray 2400sz)
+            (Rust_primitives.unsize (Libcrux.Kem.Kyber768.Parameters.Hash_functions.v_H (Rust_primitives.unsize
+                        self.Libcrux.Kem.Kyber768.Ind_cpa.KeyPair.f_pk
+                      <:
+                      slice u8)
+                  <:
+                  array u8 32sz)
+              <:
+              slice u8)
+          <:
+          Libcrux.Kem.Kyber768.Conversions.t_UpdatableArray 2400sz)
+        implicit_rejection_value
+      <:
+      Libcrux.Kem.Kyber768.Conversions.t_UpdatableArray 2400sz)
+
+let pk_under_impl (self: t_KeyPair) : array u8 1184sz =
+  self.Libcrux.Kem.Kyber768.Ind_cpa.KeyPair.f_pk
+
+let sample_matrix_A (seed: array u8 34sz) (transpose: bool)
+    : (array (array Libcrux.Kem.Kyber768.Arithmetic.t_KyberPolynomialRingElement 3sz) 3sz &
+      Core.Option.t_Option Libcrux.Kem.Kyber768.t_BadRejectionSamplingRandomnessError) =
+  let v_A_transpose:array (array Libcrux.Kem.Kyber768.Arithmetic.t_KyberPolynomialRingElement 3sz)
+    3sz =
+    Rust_primitives.Hax.repeat (Rust_primitives.Hax.repeat Libcrux.Kem.Kyber768.Arithmetic.v_ZERO_under_impl
+          3sz
+        <:
+        array Libcrux.Kem.Kyber768.Arithmetic.t_KyberPolynomialRingElement 3sz)
+      3sz
+  in
+  let sampling_A_error:Core.Option.t_Option
+  Libcrux.Kem.Kyber768.t_BadRejectionSamplingRandomnessError =
+    Core.Option.Option_None
+  in
+  let v_A_transpose, sampling_A_error, seed:(array
+      (array Libcrux.Kem.Kyber768.Arithmetic.t_KyberPolynomialRingElement 3sz) 3sz &
+    Core.Option.t_Option Libcrux.Kem.Kyber768.t_BadRejectionSamplingRandomnessError &
+    array u8 34sz) =
+    Core.Iter.Traits.Iterator.Iterator.fold (Core.Iter.Traits.Collect.IntoIterator.into_iter ({
+              Core.Ops.Range.Range.f_start = 0sz;
+              Core.Ops.Range.Range.f_end = Libcrux.Kem.Kyber768.Parameters.v_RANK
+            })
+        <:
+        _)
+      (v_A_transpose, sampling_A_error, seed)
+      (fun (v_A_transpose, sampling_A_error, seed) i ->
+          Core.Iter.Traits.Iterator.Iterator.fold (Core.Iter.Traits.Collect.IntoIterator.into_iter ({
+                    Core.Ops.Range.Range.f_start = 0sz;
+                    Core.Ops.Range.Range.f_end = Libcrux.Kem.Kyber768.Parameters.v_RANK
+                  })
+              <:
+              _)
+            (v_A_transpose, sampling_A_error, seed)
+            (fun (v_A_transpose, sampling_A_error, seed) j ->
+                let seed:array u8 34sz = Rust_primitives.Hax.update_at seed 32sz (cast i) in
+                let seed:array u8 34sz = Rust_primitives.Hax.update_at seed 33sz (cast j) in
+                let (xof_bytes: array u8 840sz):array u8 840sz =
+                  Libcrux.Kem.Kyber768.Parameters.Hash_functions.v_XOF (Rust_primitives.unsize seed
+                      <:
+                      slice u8)
+                in
+                let sampled, error:(Libcrux.Kem.Kyber768.Arithmetic.t_KyberPolynomialRingElement &
+                  Core.Option.t_Option Libcrux.Kem.Kyber768.t_BadRejectionSamplingRandomnessError) =
+                  Libcrux.Kem.Kyber768.Sampling.sample_from_uniform_distribution xof_bytes
+                in
+                let sampling_A_error:Core.Option.t_Option
+                Libcrux.Kem.Kyber768.t_BadRejectionSamplingRandomnessError =
+                  if Core.Option.is_some_under_impl error
+                  then
+                    let sampling_A_error:Core.Option.t_Option
+                    Libcrux.Kem.Kyber768.t_BadRejectionSamplingRandomnessError =
+                      error
+                    in
+                    sampling_A_error
+                  else sampling_A_error
+                in
+                if transpose
+                then
+                  let v_A_transpose:array
+                    (array Libcrux.Kem.Kyber768.Arithmetic.t_KyberPolynomialRingElement 3sz) 3sz =
+                    Rust_primitives.Hax.update_at v_A_transpose
+                      j
+                      (Rust_primitives.Hax.update_at (v_A_transpose.[ j ]
+                            <:
+                            array Libcrux.Kem.Kyber768.Arithmetic.t_KyberPolynomialRingElement 3sz)
+                          i
+                          sampled
+                        <:
+                        array Libcrux.Kem.Kyber768.Arithmetic.t_KyberPolynomialRingElement 3sz)
+                  in
+                  v_A_transpose, sampling_A_error, seed
+                else
+                  let v_A_transpose:array
+                    (array Libcrux.Kem.Kyber768.Arithmetic.t_KyberPolynomialRingElement 3sz) 3sz =
+                    Rust_primitives.Hax.update_at v_A_transpose
+                      i
+                      (Rust_primitives.Hax.update_at (v_A_transpose.[ i ]
+                            <:
+                            array Libcrux.Kem.Kyber768.Arithmetic.t_KyberPolynomialRingElement 3sz)
+                          j
+                          sampled
+                        <:
+                        array Libcrux.Kem.Kyber768.Arithmetic.t_KyberPolynomialRingElement 3sz)
+                  in
+                  v_A_transpose, sampling_A_error, seed)
+          <:
+          (array (array Libcrux.Kem.Kyber768.Arithmetic.t_KyberPolynomialRingElement 3sz) 3sz &
+            Core.Option.t_Option Libcrux.Kem.Kyber768.t_BadRejectionSamplingRandomnessError &
+            array u8 34sz))
+  in
+  v_A_transpose, sampling_A_error
+
+let cbd (prf_input: array u8 33sz)
+    : (array Libcrux.Kem.Kyber768.Arithmetic.t_KyberPolynomialRingElement 3sz & u8) =
+  let domain_separator:u8 = 0uy in
+  let re_as_ntt:array Libcrux.Kem.Kyber768.Arithmetic.t_KyberPolynomialRingElement 3sz =
+    Rust_primitives.Hax.repeat Libcrux.Kem.Kyber768.Arithmetic.v_ZERO_under_impl 3sz
+  in
+  let domain_separator, prf_input, re_as_ntt:(Prims.unit & array u8 33sz &
+    array Libcrux.Kem.Kyber768.Arithmetic.t_KyberPolynomialRingElement 3sz) =
+    Core.Iter.Traits.Iterator.Iterator.fold (Core.Iter.Traits.Collect.IntoIterator.into_iter ({
+              Core.Ops.Range.Range.f_start = 0sz;
+              Core.Ops.Range.Range.f_end = Libcrux.Kem.Kyber768.Parameters.v_RANK
+            })
+        <:
+        _)
+      (domain_separator, prf_input, re_as_ntt)
+      (fun (domain_separator, prf_input, re_as_ntt) i ->
+          let prf_input:array u8 33sz =
+            Rust_primitives.Hax.update_at prf_input 32sz domain_separator
+          in
+          let domain_separator:Prims.unit = domain_separator +. 1uy in
+          let (prf_output: array u8 128sz):array u8 128sz =
+            Libcrux.Kem.Kyber768.Parameters.Hash_functions.v_PRF (Rust_primitives.unsize prf_input
+                <:
+                slice u8)
+          in
+          let r:Libcrux.Kem.Kyber768.Arithmetic.t_KyberPolynomialRingElement =
+            Libcrux.Kem.Kyber768.Sampling.sample_from_binomial_distribution_2_ prf_output
+          in
+          let re_as_ntt:array Libcrux.Kem.Kyber768.Arithmetic.t_KyberPolynomialRingElement 3sz =
+            Rust_primitives.Hax.update_at re_as_ntt
+              i
+              (Libcrux.Kem.Kyber768.Ntt.Kyber_polynomial_ring_element_mod.ntt_representation r
+                <:
+                Libcrux.Kem.Kyber768.Arithmetic.t_KyberPolynomialRingElement)
+          in
+          domain_separator, prf_input, re_as_ntt)
+  in
+  re_as_ntt, domain_separator
+
+let encode_12_ (input: array Libcrux.Kem.Kyber768.Arithmetic.t_KyberPolynomialRingElement 3sz)
+    : array u8 1152sz =
+  let out:array u8 1152sz = Rust_primitives.Hax.repeat 0uy 1152sz in
+  let out:array u8 1152sz =
+    Core.Iter.Traits.Iterator.Iterator.fold (Core.Iter.Traits.Collect.IntoIterator.into_iter (Core.Iter.Traits.Iterator.Iterator.enumerate
+              (Core.Iter.Traits.Collect.IntoIterator.into_iter input <: _)
+            <:
+            Core.Iter.Adapters.Enumerate.t_Enumerate
+            (Core.Array.Iter.t_IntoIter Libcrux.Kem.Kyber768.Arithmetic.t_KyberPolynomialRingElement
+                3sz))
+        <:
+        _)
+      out
+      (fun out (i, re) ->
+          Rust_primitives.Hax.update_at out
+            ({
+                Core.Ops.Range.Range.f_start
+                =
+                i *. Libcrux.Kem.Kyber768.Parameters.v_BYTES_PER_RING_ELEMENT <: usize;
+                Core.Ops.Range.Range.f_end
+                =
+                (i +. 1sz <: usize) *. Libcrux.Kem.Kyber768.Parameters.v_BYTES_PER_RING_ELEMENT
+                <:
+                usize
+              })
+            (Core.Slice.copy_from_slice_under_impl (Core.Ops.Index.IndexMut.index_mut out
+                    ({
+                        Core.Ops.Range.Range.f_start
+                        =
+                        i *. Libcrux.Kem.Kyber768.Parameters.v_BYTES_PER_RING_ELEMENT <: usize;
+                        Core.Ops.Range.Range.f_end
+                        =
+                        (i +. 1sz <: usize) *.
+                        Libcrux.Kem.Kyber768.Parameters.v_BYTES_PER_RING_ELEMENT
+                        <:
+                        usize
+                      })
+                  <:
+                  slice u8)
+                (Rust_primitives.unsize (Libcrux.Kem.Kyber768.Serialize.serialize_little_endian_12_ re
+
+                      <:
+                      array u8 384sz)
+                  <:
+                  slice u8)
+              <:
+              slice u8)
+          <:
+          array u8 1152sz)
+  in
+  out
+
+let generate_keypair (key_generation_seed: slice u8)
+    : (t_KeyPair & Core.Option.t_Option Libcrux.Kem.Kyber768.t_BadRejectionSamplingRandomnessError) =
+  let (prf_input: array u8 33sz):array u8 33sz = Rust_primitives.Hax.repeat 0uy 33sz in
+  let secret_as_ntt:array Libcrux.Kem.Kyber768.Arithmetic.t_KyberPolynomialRingElement 3sz =
+    Rust_primitives.Hax.repeat Libcrux.Kem.Kyber768.Arithmetic.v_ZERO_under_impl 3sz
+  in
+  let error_as_ntt:array Libcrux.Kem.Kyber768.Arithmetic.t_KyberPolynomialRingElement 3sz =
+    Rust_primitives.Hax.repeat Libcrux.Kem.Kyber768.Arithmetic.v_ZERO_under_impl 3sz
+  in
+  let (domain_separator: u8):u8 = 0uy in
+  let hashed:array u8 64sz =
+    Libcrux.Kem.Kyber768.Parameters.Hash_functions.v_G key_generation_seed
+  in
+  let seed_for_A, seed_for_secret_and_error:(slice u8 & slice u8) =
+    Core.Slice.split_at_under_impl (Rust_primitives.unsize hashed <: slice u8) 32sz
+  in
+  let v_A_transpose, sampling_A_error:(array
+      (array Libcrux.Kem.Kyber768.Arithmetic.t_KyberPolynomialRingElement 3sz) 3sz &
+    Core.Option.t_Option Libcrux.Kem.Kyber768.t_BadRejectionSamplingRandomnessError) =
+    sample_matrix_A (Libcrux.Kem.Kyber768.Conversions.into_padded_array seed_for_A <: array u8 34sz)
+      true
+  in
+  let prf_input:array u8 33sz =
+    Rust_primitives.Hax.update_at prf_input
+      ({
+          Core.Ops.Range.Range.f_start = 0sz;
+          Core.Ops.Range.Range.f_end = Core.Slice.len_under_impl seed_for_secret_and_error <: usize
+        })
+      (Core.Slice.copy_from_slice_under_impl (Core.Ops.Index.IndexMut.index_mut prf_input
+              ({
+                  Core.Ops.Range.Range.f_start = 0sz;
+                  Core.Ops.Range.Range.f_end
+                  =
+                  Core.Slice.len_under_impl seed_for_secret_and_error <: usize
+                })
+            <:
+            slice u8)
+          seed_for_secret_and_error
+        <:
+        slice u8)
+  in
+  let domain_separator, prf_input, secret_as_ntt:(Prims.unit & array u8 33sz &
+    array Libcrux.Kem.Kyber768.Arithmetic.t_KyberPolynomialRingElement 3sz) =
+    Core.Iter.Traits.Iterator.Iterator.fold (Core.Iter.Traits.Collect.IntoIterator.into_iter ({
+              Core.Ops.Range.Range.f_start = 0sz;
+              Core.Ops.Range.Range.f_end = Libcrux.Kem.Kyber768.Parameters.v_RANK
+            })
+        <:
+        _)
+      (domain_separator, prf_input, secret_as_ntt)
+      (fun (domain_separator, prf_input, secret_as_ntt) i ->
+          let prf_input:array u8 33sz =
+            Rust_primitives.Hax.update_at prf_input 32sz domain_separator
+          in
+          let domain_separator:Prims.unit = domain_separator +. 1uy in
+          let (prf_output: array u8 128sz):array u8 128sz =
+            Libcrux.Kem.Kyber768.Parameters.Hash_functions.v_PRF (Rust_primitives.unsize prf_input
+                <:
+                slice u8)
+          in
+          let secret:Libcrux.Kem.Kyber768.Arithmetic.t_KyberPolynomialRingElement =
+            Libcrux.Kem.Kyber768.Sampling.sample_from_binomial_distribution_2_ prf_output
+          in
+          let secret_as_ntt:array Libcrux.Kem.Kyber768.Arithmetic.t_KyberPolynomialRingElement 3sz =
+            Rust_primitives.Hax.update_at secret_as_ntt
+              i
+              (Libcrux.Kem.Kyber768.Ntt.Kyber_polynomial_ring_element_mod.ntt_representation secret
+                <:
+                Libcrux.Kem.Kyber768.Arithmetic.t_KyberPolynomialRingElement)
+          in
+          domain_separator, prf_input, secret_as_ntt)
+  in
+  let domain_separator, error_as_ntt, prf_input:(Prims.unit &
+    array Libcrux.Kem.Kyber768.Arithmetic.t_KyberPolynomialRingElement 3sz &
+    array u8 33sz) =
+    Core.Iter.Traits.Iterator.Iterator.fold (Core.Iter.Traits.Collect.IntoIterator.into_iter ({
+              Core.Ops.Range.Range.f_start = 0sz;
+              Core.Ops.Range.Range.f_end = Libcrux.Kem.Kyber768.Parameters.v_RANK
+            })
+        <:
+        _)
+      (domain_separator, error_as_ntt, prf_input)
+      (fun (domain_separator, error_as_ntt, prf_input) i ->
+          let prf_input:array u8 33sz =
+            Rust_primitives.Hax.update_at prf_input 32sz domain_separator
+          in
+          let domain_separator:Prims.unit = domain_separator +. 1uy in
+          let (prf_output: array u8 128sz):array u8 128sz =
+            Libcrux.Kem.Kyber768.Parameters.Hash_functions.v_PRF (Rust_primitives.unsize prf_input
+                <:
+                slice u8)
+          in
+          let error:Libcrux.Kem.Kyber768.Arithmetic.t_KyberPolynomialRingElement =
+            Libcrux.Kem.Kyber768.Sampling.sample_from_binomial_distribution_2_ prf_output
+          in
+          let error_as_ntt:array Libcrux.Kem.Kyber768.Arithmetic.t_KyberPolynomialRingElement 3sz =
+            Rust_primitives.Hax.update_at error_as_ntt
+              i
+              (Libcrux.Kem.Kyber768.Ntt.Kyber_polynomial_ring_element_mod.ntt_representation error
+                <:
+                Libcrux.Kem.Kyber768.Arithmetic.t_KyberPolynomialRingElement)
+          in
+          domain_separator, error_as_ntt, prf_input)
+  in
+  let t__as_ntt:array Libcrux.Kem.Kyber768.Arithmetic.t_KyberPolynomialRingElement 3sz =
+    Libcrux.Kem.Kyber768.Ntt.multiply_matrix_by_column v_A_transpose secret_as_ntt
+  in
+  let t__as_ntt:array Libcrux.Kem.Kyber768.Arithmetic.t_KyberPolynomialRingElement 3sz =
+    Core.Iter.Traits.Iterator.Iterator.fold (Core.Iter.Traits.Collect.IntoIterator.into_iter ({
+              Core.Ops.Range.Range.f_start = 0sz;
+              Core.Ops.Range.Range.f_end = Libcrux.Kem.Kyber768.Parameters.v_RANK
+            })
+        <:
+        _)
+      t__as_ntt
+      (fun t__as_ntt i ->
+          Rust_primitives.Hax.update_at t__as_ntt
+            i
+            ((t__as_ntt.[ i ] <: Libcrux.Kem.Kyber768.Arithmetic.t_KyberPolynomialRingElement) +.
+              (error_as_ntt.[ i ] <: Libcrux.Kem.Kyber768.Arithmetic.t_KyberPolynomialRingElement)
+              <:
+              _)
+          <:
+          array Libcrux.Kem.Kyber768.Arithmetic.t_KyberPolynomialRingElement 3sz)
+  in
+  let public_key_serialized:array u8 1184sz =
+    Libcrux.Kem.Kyber768.Conversions.array_under_impl (Libcrux.Kem.Kyber768.Conversions.UpdatingArray.push
+          (Libcrux.Kem.Kyber768.Conversions.UpdatingArray.push (Libcrux.Kem.Kyber768.Conversions.new_under_impl
+                  (Rust_primitives.Hax.repeat 0uy 1184sz <: array u8 1184sz)
+                <:
+                Libcrux.Kem.Kyber768.Conversions.t_UpdatableArray 1184sz)
+              (Rust_primitives.unsize (encode_12_ t__as_ntt <: array u8 1152sz) <: slice u8)
+            <:
+            Libcrux.Kem.Kyber768.Conversions.t_UpdatableArray 1184sz)
+          seed_for_A
+        <:
+        Libcrux.Kem.Kyber768.Conversions.t_UpdatableArray 1184sz)
+  in
+  let secret_key_serialized:array u8 1152sz = encode_12_ secret_as_ntt in
+  new_under_impl secret_key_serialized public_key_serialized, sampling_A_error
+
+let compress_then_encode_u
+      (input: array Libcrux.Kem.Kyber768.Arithmetic.t_KyberPolynomialRingElement 3sz)
+    : array u8 960sz =
+  let out:array u8 960sz = Rust_primitives.Hax.repeat 0uy 960sz in
+  let out:array u8 960sz =
+    Core.Iter.Traits.Iterator.Iterator.fold (Core.Iter.Traits.Collect.IntoIterator.into_iter (Core.Iter.Traits.Iterator.Iterator.enumerate
+              (Core.Iter.Traits.Collect.IntoIterator.into_iter input <: _)
+            <:
+            Core.Iter.Adapters.Enumerate.t_Enumerate
+            (Core.Array.Iter.t_IntoIter Libcrux.Kem.Kyber768.Arithmetic.t_KyberPolynomialRingElement
+                3sz))
+        <:
+        _)
+      out
+      (fun out (i, re) ->
+          Rust_primitives.Hax.update_at out
+            ({
+                Core.Ops.Range.Range.f_start
+                =
+                i *. Libcrux.Kem.Kyber768.Parameters.v_BYTES_PER_ENCODED_ELEMENT_OF_U <: usize;
+                Core.Ops.Range.Range.f_end
+                =
+                (i +. 1sz <: usize) *.
+                Libcrux.Kem.Kyber768.Parameters.v_BYTES_PER_ENCODED_ELEMENT_OF_U
+                <:
+                usize
+              })
+            (Core.Slice.copy_from_slice_under_impl (Core.Ops.Index.IndexMut.index_mut out
+                    ({
+                        Core.Ops.Range.Range.f_start
+                        =
+                        i *. Libcrux.Kem.Kyber768.Parameters.v_BYTES_PER_ENCODED_ELEMENT_OF_U
+                        <:
+                        usize;
+                        Core.Ops.Range.Range.f_end
+                        =
+                        (i +. 1sz <: usize) *.
+                        Libcrux.Kem.Kyber768.Parameters.v_BYTES_PER_ENCODED_ELEMENT_OF_U
+                        <:
+                        usize
+                      })
+                  <:
+                  slice u8)
+                (Rust_primitives.unsize (Libcrux.Kem.Kyber768.Serialize.serialize_little_endian_10_ (
+                          Libcrux.Kem.Kyber768.Compress.compress re
+                            Libcrux.Kem.Kyber768.Parameters.v_VECTOR_U_COMPRESSION_FACTOR
+                          <:
+                          Libcrux.Kem.Kyber768.Arithmetic.t_KyberPolynomialRingElement)
+                      <:
+                      array u8 320sz)
+                  <:
+                  slice u8)
+              <:
+              slice u8)
+          <:
+          array u8 960sz)
+  in
+  out
+
+let encrypt (public_key: slice u8) (message: array u8 32sz) (randomness: slice u8)
+    : (array u8 1088sz &
+      Core.Option.t_Option Libcrux.Kem.Kyber768.t_BadRejectionSamplingRandomnessError) =
+  let t__as_ntt:array Libcrux.Kem.Kyber768.Arithmetic.t_KyberPolynomialRingElement 3sz =
+    Rust_primitives.Hax.repeat Libcrux.Kem.Kyber768.Arithmetic.v_ZERO_under_impl 3sz
+  in
+  let t__as_ntt:array Libcrux.Kem.Kyber768.Arithmetic.t_KyberPolynomialRingElement 3sz =
+    Core.Iter.Traits.Iterator.Iterator.fold (Core.Iter.Traits.Collect.IntoIterator.into_iter (Core.Iter.Traits.Iterator.Iterator.enumerate
+              (Core.Slice.chunks_exact_under_impl (public_key.[ {
+                        Core.Ops.Range.RangeTo.f_end
+                        =
+                        Libcrux.Kem.Kyber768.Parameters.v_T_AS_NTT_ENCODED_SIZE
+                      } ]
+                    <:
+                    slice u8)
+                  Libcrux.Kem.Kyber768.Parameters.v_BYTES_PER_RING_ELEMENT
+                <:
+                Core.Slice.Iter.t_ChunksExact u8)
+            <:
+            Core.Iter.Adapters.Enumerate.t_Enumerate (Core.Slice.Iter.t_ChunksExact u8))
+        <:
+        _)
+      t__as_ntt
+      (fun t__as_ntt (i, t__as_ntt_bytes) ->
+          Rust_primitives.Hax.update_at t__as_ntt
+            i
+            (Libcrux.Kem.Kyber768.Serialize.deserialize_little_endian_12_ t__as_ntt_bytes
+              <:
+              Libcrux.Kem.Kyber768.Arithmetic.t_KyberPolynomialRingElement)
+          <:
+          array Libcrux.Kem.Kyber768.Arithmetic.t_KyberPolynomialRingElement 3sz)
+  in
+  let seed:slice u8 =
+    public_key.[ {
+        Core.Ops.Range.RangeFrom.f_start = Libcrux.Kem.Kyber768.Parameters.v_T_AS_NTT_ENCODED_SIZE
+      } ]
+  in
+  let v_A_transpose, sampling_A_error:(array
+      (array Libcrux.Kem.Kyber768.Arithmetic.t_KyberPolynomialRingElement 3sz) 3sz &
+    Core.Option.t_Option Libcrux.Kem.Kyber768.t_BadRejectionSamplingRandomnessError) =
+    sample_matrix_A (Libcrux.Kem.Kyber768.Conversions.into_padded_array seed <: array u8 34sz) false
+  in
+  let (prf_input: array u8 33sz):array u8 33sz =
+    Libcrux.Kem.Kyber768.Conversions.into_padded_array randomness
+  in
+  let r_as_ntt, domain_separator:(array Libcrux.Kem.Kyber768.Arithmetic.t_KyberPolynomialRingElement
+      3sz &
+    u8) =
+    cbd prf_input
+  in
+  let error_1_:array Libcrux.Kem.Kyber768.Arithmetic.t_KyberPolynomialRingElement 3sz =
+    Rust_primitives.Hax.repeat Libcrux.Kem.Kyber768.Arithmetic.v_ZERO_under_impl 3sz
+  in
+  let domain_separator, error_1_, prf_input:(Prims.unit &
+    array Libcrux.Kem.Kyber768.Arithmetic.t_KyberPolynomialRingElement 3sz &
+    array u8 33sz) =
+    Core.Iter.Traits.Iterator.Iterator.fold (Core.Iter.Traits.Collect.IntoIterator.into_iter ({
+              Core.Ops.Range.Range.f_start = 0sz;
+              Core.Ops.Range.Range.f_end = Libcrux.Kem.Kyber768.Parameters.v_RANK
+            })
+        <:
+        _)
+      (domain_separator, error_1_, prf_input)
+      (fun (domain_separator, error_1_, prf_input) i ->
+          let prf_input:array u8 33sz =
+            Rust_primitives.Hax.update_at prf_input 32sz domain_separator
+          in
+          let domain_separator:Prims.unit = domain_separator +. 1uy in
+          let (prf_output: array u8 128sz):array u8 128sz =
+            Libcrux.Kem.Kyber768.Parameters.Hash_functions.v_PRF (Rust_primitives.unsize prf_input
+                <:
+                slice u8)
+          in
+          let error_1_:array Libcrux.Kem.Kyber768.Arithmetic.t_KyberPolynomialRingElement 3sz =
+            Rust_primitives.Hax.update_at error_1_
+              i
+              (Libcrux.Kem.Kyber768.Sampling.sample_from_binomial_distribution_2_ prf_output
+                <:
+                Libcrux.Kem.Kyber768.Arithmetic.t_KyberPolynomialRingElement)
+          in
+          domain_separator, error_1_, prf_input)
+  in
+  let prf_input:array u8 33sz = Rust_primitives.Hax.update_at prf_input 32sz domain_separator in
+  let (prf_output: array u8 128sz):array u8 128sz =
+    Libcrux.Kem.Kyber768.Parameters.Hash_functions.v_PRF (Rust_primitives.unsize prf_input
+        <:
+        slice u8)
+  in
+  let error_2_:Libcrux.Kem.Kyber768.Arithmetic.t_KyberPolynomialRingElement =
+    Libcrux.Kem.Kyber768.Sampling.sample_from_binomial_distribution_2_ prf_output
+  in
+  let u:array Libcrux.Kem.Kyber768.Arithmetic.t_KyberPolynomialRingElement 3sz =
+    Libcrux.Kem.Kyber768.Ntt.multiply_matrix_by_column_montgomery v_A_transpose r_as_ntt
+  in
+  let u:array Libcrux.Kem.Kyber768.Arithmetic.t_KyberPolynomialRingElement 3sz =
+    Core.Iter.Traits.Iterator.Iterator.fold (Core.Iter.Traits.Collect.IntoIterator.into_iter ({
+              Core.Ops.Range.Range.f_start = 0sz;
+              Core.Ops.Range.Range.f_end = Libcrux.Kem.Kyber768.Parameters.v_RANK
+            })
+        <:
+        _)
+      u
+      (fun u i ->
+          Rust_primitives.Hax.update_at u
+            i
+            ((Libcrux.Kem.Kyber768.Ntt.Kyber_polynomial_ring_element_mod.invert_ntt_montgomery (u.[ i
+                    ]
+                    <:
+                    Libcrux.Kem.Kyber768.Arithmetic.t_KyberPolynomialRingElement)
+                <:
+                Libcrux.Kem.Kyber768.Arithmetic.t_KyberPolynomialRingElement) +.
+              (error_1_.[ i ] <: Libcrux.Kem.Kyber768.Arithmetic.t_KyberPolynomialRingElement)
+              <:
+              _)
+          <:
+          array Libcrux.Kem.Kyber768.Arithmetic.t_KyberPolynomialRingElement 3sz)
+  in
+  let message_as_ring_element:Libcrux.Kem.Kyber768.Arithmetic.t_KyberPolynomialRingElement =
+    Libcrux.Kem.Kyber768.Serialize.deserialize_little_endian_1_ (Rust_primitives.unsize message
+        <:
+        slice u8)
+  in
+  let v =
+    ((Libcrux.Kem.Kyber768.Ntt.Kyber_polynomial_ring_element_mod.invert_ntt_montgomery (Libcrux.Kem.Kyber768.Ntt.multiply_row_by_column_montgomery
+              t__as_ntt
+              r_as_ntt
+            <:
+            Libcrux.Kem.Kyber768.Arithmetic.t_KyberPolynomialRingElement)
+        <:
+        Libcrux.Kem.Kyber768.Arithmetic.t_KyberPolynomialRingElement) +.
+      error_2_
+      <:
+      _) +.
+    (Libcrux.Kem.Kyber768.Compress.decompress message_as_ring_element 1sz
+      <:
+      Libcrux.Kem.Kyber768.Arithmetic.t_KyberPolynomialRingElement)
+  in
+  let c1:array u8 960sz = compress_then_encode_u u in
+  let c2:array u8 128sz =
+    Libcrux.Kem.Kyber768.Serialize.serialize_little_endian_4_ (Libcrux.Kem.Kyber768.Compress.compress
+          v
+          Libcrux.Kem.Kyber768.Parameters.v_VECTOR_V_COMPRESSION_FACTOR
+        <:
+        Libcrux.Kem.Kyber768.Arithmetic.t_KyberPolynomialRingElement)
+  in
+  let (ciphertext: array u8 1088sz):array u8 1088sz =
+    Libcrux.Kem.Kyber768.Conversions.into_padded_array (Rust_primitives.unsize c1 <: slice u8)
+  in
+  let ciphertext:array u8 1088sz =
+    Rust_primitives.Hax.update_at ciphertext
+      ({
+          Core.Ops.Range.RangeFrom.f_start = Libcrux.Kem.Kyber768.Parameters.v_VECTOR_U_ENCODED_SIZE
+        })
+      (Core.Slice.copy_from_slice_under_impl (Core.Ops.Index.IndexMut.index_mut ciphertext
+              ({
+                  Core.Ops.Range.RangeFrom.f_start
+                  =
+                  Libcrux.Kem.Kyber768.Parameters.v_VECTOR_U_ENCODED_SIZE
+                })
+            <:
+            slice u8)
+          (Core.Array.as_slice_under_impl_23 c2 <: slice u8)
+        <:
+        slice u8)
+  in
+  ciphertext, sampling_A_error
+
+let decrypt (secret_key: slice u8) (ciphertext: array u8 1088sz) : array u8 32sz =
+  let u_as_ntt:array Libcrux.Kem.Kyber768.Arithmetic.t_KyberPolynomialRingElement 3sz =
+    Rust_primitives.Hax.repeat Libcrux.Kem.Kyber768.Arithmetic.v_ZERO_under_impl 3sz
+  in
+  let secret_as_ntt:array Libcrux.Kem.Kyber768.Arithmetic.t_KyberPolynomialRingElement 3sz =
+    Rust_primitives.Hax.repeat Libcrux.Kem.Kyber768.Arithmetic.v_ZERO_under_impl 3sz
+  in
+  let u_as_ntt:array Libcrux.Kem.Kyber768.Arithmetic.t_KyberPolynomialRingElement 3sz =
+    Core.Iter.Traits.Iterator.Iterator.fold (Core.Iter.Traits.Collect.IntoIterator.into_iter (Core.Iter.Traits.Iterator.Iterator.enumerate
+              (Core.Slice.chunks_exact_under_impl (ciphertext.[ {
+                        Core.Ops.Range.RangeTo.f_end
+                        =
+                        Libcrux.Kem.Kyber768.Parameters.v_VECTOR_U_ENCODED_SIZE
+                      } ]
+                    <:
+                    slice u8)
+                  ((Libcrux.Kem.Kyber768.Parameters.v_COEFFICIENTS_IN_RING_ELEMENT *. 10sz <: usize) /.
+                    8sz
+                    <:
+                    usize)
+                <:
+                Core.Slice.Iter.t_ChunksExact u8)
+            <:
+            Core.Iter.Adapters.Enumerate.t_Enumerate (Core.Slice.Iter.t_ChunksExact u8))
+        <:
+        _)
+      u_as_ntt
+      (fun u_as_ntt (i, u_bytes) ->
+          let u:Libcrux.Kem.Kyber768.Arithmetic.t_KyberPolynomialRingElement =
+            Libcrux.Kem.Kyber768.Serialize.deserialize_little_endian_10_ u_bytes
+          in
+          let u_as_ntt:array Libcrux.Kem.Kyber768.Arithmetic.t_KyberPolynomialRingElement 3sz =
+            Rust_primitives.Hax.update_at u_as_ntt
+              i
+              (Libcrux.Kem.Kyber768.Ntt.Kyber_polynomial_ring_element_mod.ntt_representation (Libcrux.Kem.Kyber768.Compress.decompress
+                      u
+                      10sz
+                    <:
+                    Libcrux.Kem.Kyber768.Arithmetic.t_KyberPolynomialRingElement)
+                <:
+                Libcrux.Kem.Kyber768.Arithmetic.t_KyberPolynomialRingElement)
+          in
+          u_as_ntt)
+  in
+  let v:Libcrux.Kem.Kyber768.Arithmetic.t_KyberPolynomialRingElement =
+    Libcrux.Kem.Kyber768.Compress.decompress (Libcrux.Kem.Kyber768.Serialize.deserialize_little_endian_4_
+          (ciphertext.[ {
+                Core.Ops.Range.RangeFrom.f_start
+                =
+                Libcrux.Kem.Kyber768.Parameters.v_VECTOR_U_ENCODED_SIZE
+              } ]
+            <:
+            slice u8)
+        <:
+        Libcrux.Kem.Kyber768.Arithmetic.t_KyberPolynomialRingElement)
+      Libcrux.Kem.Kyber768.Parameters.v_VECTOR_V_COMPRESSION_FACTOR
+  in
+  let secret_as_ntt:array Libcrux.Kem.Kyber768.Arithmetic.t_KyberPolynomialRingElement 3sz =
+    Core.Iter.Traits.Iterator.Iterator.fold (Core.Iter.Traits.Collect.IntoIterator.into_iter (Core.Iter.Traits.Iterator.Iterator.enumerate
+              (Core.Slice.chunks_exact_under_impl secret_key
+                  Libcrux.Kem.Kyber768.Parameters.v_BYTES_PER_RING_ELEMENT
+                <:
+                Core.Slice.Iter.t_ChunksExact u8)
+            <:
+            Core.Iter.Adapters.Enumerate.t_Enumerate (Core.Slice.Iter.t_ChunksExact u8))
+        <:
+        _)
+      secret_as_ntt
+      (fun secret_as_ntt (i, secret_bytes) ->
+          Rust_primitives.Hax.update_at secret_as_ntt
+            i
+            (Libcrux.Kem.Kyber768.Serialize.deserialize_little_endian_12_ secret_bytes
+              <:
+              Libcrux.Kem.Kyber768.Arithmetic.t_KyberPolynomialRingElement)
+          <:
+          array Libcrux.Kem.Kyber768.Arithmetic.t_KyberPolynomialRingElement 3sz)
+  in
+  let message =
+    v -.
+    (Libcrux.Kem.Kyber768.Ntt.Kyber_polynomial_ring_element_mod.invert_ntt_montgomery (Libcrux.Kem.Kyber768.Ntt.multiply_row_by_column_montgomery
+            secret_as_ntt
+            u_as_ntt
+          <:
+          Libcrux.Kem.Kyber768.Arithmetic.t_KyberPolynomialRingElement)
+      <:
+      Libcrux.Kem.Kyber768.Arithmetic.t_KyberPolynomialRingElement)
+  in
+  Libcrux.Kem.Kyber768.Serialize.serialize_little_endian_1_ (Libcrux.Kem.Kyber768.Compress.compress message
+        1sz
+      <:
+      Libcrux.Kem.Kyber768.Arithmetic.t_KyberPolynomialRingElement)
