examples/kyber/Libcrux.Kem.Kyber768.Ntt.fst
@@ -1,0 +1,206 @@
+module Libcrux.Kem.Kyber768.Ntt
+#set-options "--fuel 0 --ifuel 1 --z3rlimit 15"
+open Core
+
+let multiply_row_by_column_montgomery
+      (row_vector column_vector:
+          array Libcrux.Kem.Kyber768.Arithmetic.t_KyberPolynomialRingElement 3sz)
+    : Libcrux.Kem.Kyber768.Arithmetic.t_KyberPolynomialRingElement =
+  let result:Libcrux.Kem.Kyber768.Arithmetic.t_KyberPolynomialRingElement =
+    Libcrux.Kem.Kyber768.Arithmetic.v_ZERO_under_impl
+  in
+  let result =
+    Core.Iter.Traits.Iterator.Iterator.fold (Core.Iter.Traits.Collect.IntoIterator.into_iter (Core.Iter.Traits.Iterator.Iterator.zip
+              (Core.Slice.iter_under_impl (Rust_primitives.unsize row_vector
+                    <:
+                    slice Libcrux.Kem.Kyber768.Arithmetic.t_KyberPolynomialRingElement)
+                <:
+                Core.Slice.Iter.t_Iter Libcrux.Kem.Kyber768.Arithmetic.t_KyberPolynomialRingElement)
+              (Core.Slice.iter_under_impl (Rust_primitives.unsize column_vector
+                    <:
+                    slice Libcrux.Kem.Kyber768.Arithmetic.t_KyberPolynomialRingElement)
+                <:
+                Core.Slice.Iter.t_Iter Libcrux.Kem.Kyber768.Arithmetic.t_KyberPolynomialRingElement)
+            <:
+            Core.Iter.Adapters.Zip.t_Zip
+              (Core.Slice.Iter.t_Iter Libcrux.Kem.Kyber768.Arithmetic.t_KyberPolynomialRingElement)
+              _)
+        <:
+        _)
+      result
+      (fun result (row_element, column_element) ->
+          result +.
+          (Libcrux.Kem.Kyber768.Ntt.Kyber_polynomial_ring_element_mod.ntt_multiply row_element
+              column_element
+            <:
+            Libcrux.Kem.Kyber768.Arithmetic.t_KyberPolynomialRingElement)
+          <:
+          _)
+  in
+  let result:Libcrux.Kem.Kyber768.Arithmetic.t_KyberPolynomialRingElement =
+    {
+      result with
+      Libcrux.Kem.Kyber768.Arithmetic.KyberPolynomialRingElement.f_coefficients
+      =
+      Core.Array.map_under_impl_23 result
+          .Libcrux.Kem.Kyber768.Arithmetic.KyberPolynomialRingElement.f_coefficients
+        Libcrux.Kem.Kyber768.Arithmetic.barrett_reduce
+    }
+  in
+  result
+
+let multiply_matrix_by_column_montgomery
+      (matrix: array (array Libcrux.Kem.Kyber768.Arithmetic.t_KyberPolynomialRingElement 3sz) 3sz)
+      (vector: array Libcrux.Kem.Kyber768.Arithmetic.t_KyberPolynomialRingElement 3sz)
+    : array Libcrux.Kem.Kyber768.Arithmetic.t_KyberPolynomialRingElement 3sz =
+  let result:array Libcrux.Kem.Kyber768.Arithmetic.t_KyberPolynomialRingElement 3sz =
+    Rust_primitives.Hax.repeat Libcrux.Kem.Kyber768.Arithmetic.v_ZERO_under_impl 3sz
+  in
+  let result:array Libcrux.Kem.Kyber768.Arithmetic.t_KyberPolynomialRingElement 3sz =
+    Core.Iter.Traits.Iterator.Iterator.fold (Core.Iter.Traits.Collect.IntoIterator.into_iter (Core.Iter.Traits.Iterator.Iterator.enumerate
+              (Core.Slice.iter_under_impl (Rust_primitives.unsize matrix
+                    <:
+                    slice (array Libcrux.Kem.Kyber768.Arithmetic.t_KyberPolynomialRingElement 3sz))
+                <:
+                Core.Slice.Iter.t_Iter
+                (array Libcrux.Kem.Kyber768.Arithmetic.t_KyberPolynomialRingElement 3sz))
+            <:
+            Core.Iter.Adapters.Enumerate.t_Enumerate
+            (Core.Slice.Iter.t_Iter
+              (array Libcrux.Kem.Kyber768.Arithmetic.t_KyberPolynomialRingElement 3sz)))
+        <:
+        _)
+      result
+      (fun result (i, row) ->
+          let result:array Libcrux.Kem.Kyber768.Arithmetic.t_KyberPolynomialRingElement 3sz =
+            Core.Iter.Traits.Iterator.Iterator.fold (Core.Iter.Traits.Collect.IntoIterator.into_iter
+                  (Core.Iter.Traits.Iterator.Iterator.enumerate (Core.Slice.iter_under_impl (Rust_primitives.unsize
+                              row
+                            <:
+                            slice Libcrux.Kem.Kyber768.Arithmetic.t_KyberPolynomialRingElement)
+                        <:
+                        Core.Slice.Iter.t_Iter
+                        Libcrux.Kem.Kyber768.Arithmetic.t_KyberPolynomialRingElement)
+                    <:
+                    Core.Iter.Adapters.Enumerate.t_Enumerate
+                    (Core.Slice.Iter.t_Iter
+                      Libcrux.Kem.Kyber768.Arithmetic.t_KyberPolynomialRingElement))
+                <:
+                _)
+              result
+              (fun result (j, matrix_element) ->
+                  let product:Libcrux.Kem.Kyber768.Arithmetic.t_KyberPolynomialRingElement =
+                    Libcrux.Kem.Kyber768.Ntt.Kyber_polynomial_ring_element_mod.ntt_multiply matrix_element
+                      (vector.[ j ] <: Libcrux.Kem.Kyber768.Arithmetic.t_KyberPolynomialRingElement)
+                  in
+                  let result:array Libcrux.Kem.Kyber768.Arithmetic.t_KyberPolynomialRingElement 3sz
+                  =
+                    Rust_primitives.Hax.update_at result
+                      i
+                      ((result.[ i ] <: Libcrux.Kem.Kyber768.Arithmetic.t_KyberPolynomialRingElement
+                        ) +.
+                        product
+                        <:
+                        _)
+                  in
+                  result)
+          in
+          let result:array Libcrux.Kem.Kyber768.Arithmetic.t_KyberPolynomialRingElement 3sz =
+            Rust_primitives.Hax.update_at result
+              i
+              ({
+                  (result.[ i ] <: Libcrux.Kem.Kyber768.Arithmetic.t_KyberPolynomialRingElement) with
+                  Libcrux.Kem.Kyber768.Arithmetic.KyberPolynomialRingElement.f_coefficients
+                  =
+                  Core.Array.map_under_impl_23 (result.[ i ]
+                      <:
+                      Libcrux.Kem.Kyber768.Arithmetic.t_KyberPolynomialRingElement)
+                      .Libcrux.Kem.Kyber768.Arithmetic.KyberPolynomialRingElement.f_coefficients
+                    Libcrux.Kem.Kyber768.Arithmetic.barrett_reduce
+                  <:
+                  array i32 256sz
+                })
+          in
+          result)
+  in
+  result
+
+let multiply_matrix_by_column
+      (matrix: array (array Libcrux.Kem.Kyber768.Arithmetic.t_KyberPolynomialRingElement 3sz) 3sz)
+      (vector: array Libcrux.Kem.Kyber768.Arithmetic.t_KyberPolynomialRingElement 3sz)
+    : array Libcrux.Kem.Kyber768.Arithmetic.t_KyberPolynomialRingElement 3sz =
+  let result:array Libcrux.Kem.Kyber768.Arithmetic.t_KyberPolynomialRingElement 3sz =
+    Rust_primitives.Hax.repeat Libcrux.Kem.Kyber768.Arithmetic.v_ZERO_under_impl 3sz
+  in
+  let result:array Libcrux.Kem.Kyber768.Arithmetic.t_KyberPolynomialRingElement 3sz =
+    Core.Iter.Traits.Iterator.Iterator.fold (Core.Iter.Traits.Collect.IntoIterator.into_iter (Core.Iter.Traits.Iterator.Iterator.enumerate
+              (Core.Slice.iter_under_impl (Rust_primitives.unsize matrix
+                    <:
+                    slice (array Libcrux.Kem.Kyber768.Arithmetic.t_KyberPolynomialRingElement 3sz))
+                <:
+                Core.Slice.Iter.t_Iter
+                (array Libcrux.Kem.Kyber768.Arithmetic.t_KyberPolynomialRingElement 3sz))
+            <:
+            Core.Iter.Adapters.Enumerate.t_Enumerate
+            (Core.Slice.Iter.t_Iter
+              (array Libcrux.Kem.Kyber768.Arithmetic.t_KyberPolynomialRingElement 3sz)))
+        <:
+        _)
+      result
+      (fun result (i, row) ->
+          let result:array Libcrux.Kem.Kyber768.Arithmetic.t_KyberPolynomialRingElement 3sz =
+            Core.Iter.Traits.Iterator.Iterator.fold (Core.Iter.Traits.Collect.IntoIterator.into_iter
+                  (Core.Iter.Traits.Iterator.Iterator.enumerate (Core.Slice.iter_under_impl (Rust_primitives.unsize
+                              row
+                            <:
+                            slice Libcrux.Kem.Kyber768.Arithmetic.t_KyberPolynomialRingElement)
+                        <:
+                        Core.Slice.Iter.t_Iter
+                        Libcrux.Kem.Kyber768.Arithmetic.t_KyberPolynomialRingElement)
+                    <:
+                    Core.Iter.Adapters.Enumerate.t_Enumerate
+                    (Core.Slice.Iter.t_Iter
+                      Libcrux.Kem.Kyber768.Arithmetic.t_KyberPolynomialRingElement))
+                <:
+                _)
+              result
+              (fun result (j, matrix_element) ->
+                  let product:Libcrux.Kem.Kyber768.Arithmetic.t_KyberPolynomialRingElement =
+                    Libcrux.Kem.Kyber768.Ntt.Kyber_polynomial_ring_element_mod.ntt_multiply matrix_element
+                      (vector.[ j ] <: Libcrux.Kem.Kyber768.Arithmetic.t_KyberPolynomialRingElement)
+                  in
+                  let result:array Libcrux.Kem.Kyber768.Arithmetic.t_KyberPolynomialRingElement 3sz
+                  =
+                    Rust_primitives.Hax.update_at result
+                      i
+                      ((result.[ i ] <: Libcrux.Kem.Kyber768.Arithmetic.t_KyberPolynomialRingElement
+                        ) +.
+                        product
+                        <:
+                        _)
+                  in
+                  result)
+          in
+          let result:array Libcrux.Kem.Kyber768.Arithmetic.t_KyberPolynomialRingElement 3sz =
+            Rust_primitives.Hax.update_at result
+              i
+              ({
+                  (result.[ i ] <: Libcrux.Kem.Kyber768.Arithmetic.t_KyberPolynomialRingElement) with
+                  Libcrux.Kem.Kyber768.Arithmetic.KyberPolynomialRingElement.f_coefficients
+                  =
+                  Core.Array.map_under_impl_23 (result.[ i ]
+                      <:
+                      Libcrux.Kem.Kyber768.Arithmetic.t_KyberPolynomialRingElement)
+                      .Libcrux.Kem.Kyber768.Arithmetic.KyberPolynomialRingElement.f_coefficients
+                    (fun coefficient ->
+                        let coefficient_montgomery:i32 =
+                          Libcrux.Kem.Kyber768.Arithmetic.to_montgomery_domain coefficient
+                        in
+                        Libcrux.Kem.Kyber768.Arithmetic.barrett_reduce coefficient_montgomery)
+                  <:
+                  array i32 256sz
+                })
+          in
+          result)
+  in
+  result
