examples/kyber/Libcrux.Kem.Kyber768.Parameters.fst
@@ -1,0 +1,51 @@
+module Libcrux.Kem.Kyber768.Parameters
+#set-options "--fuel 0 --ifuel 1 --z3rlimit 15"
+open Core
+
+let v_FIELD_MODULUS: i32 = 3329l
+
+let v_BITS_PER_COEFFICIENT: usize = 12sz
+
+let v_COEFFICIENTS_IN_RING_ELEMENT: usize = 256sz
+
+let v_BITS_PER_RING_ELEMENT: usize = v_COEFFICIENTS_IN_RING_ELEMENT *. 12sz
+
+let v_BYTES_PER_RING_ELEMENT: usize = v_BITS_PER_RING_ELEMENT /. 8sz
+
+let v_REJECTION_SAMPLING_SEED_SIZE: usize = 168sz *. 5sz
+
+let v_RANK: usize = 3sz
+
+let v_T_AS_NTT_ENCODED_SIZE: usize =
+  ((v_RANK *. v_COEFFICIENTS_IN_RING_ELEMENT <: usize) *. v_BITS_PER_COEFFICIENT <: usize) /. 8sz
+
+let v_VECTOR_U_COMPRESSION_FACTOR: usize = 10sz
+
+let v_VECTOR_V_COMPRESSION_FACTOR: usize = 4sz
+
+let v_BYTES_PER_ENCODED_ELEMENT_OF_U: usize =
+  (v_COEFFICIENTS_IN_RING_ELEMENT *. v_VECTOR_U_COMPRESSION_FACTOR <: usize) /. 8sz
+
+let v_VECTOR_U_ENCODED_SIZE: usize = v_RANK *. v_BYTES_PER_ENCODED_ELEMENT_OF_U
+
+let v_VECTOR_V_ENCODED_SIZE: usize =
+  (v_COEFFICIENTS_IN_RING_ELEMENT *. v_VECTOR_V_COMPRESSION_FACTOR <: usize) /. 8sz
+
+let v_CPA_PKE_KEY_GENERATION_SEED_SIZE: usize = 32sz
+
+let v_CPA_PKE_SECRET_KEY_SIZE: usize =
+  ((v_RANK *. v_COEFFICIENTS_IN_RING_ELEMENT <: usize) *. v_BITS_PER_COEFFICIENT <: usize) /. 8sz
+
+let v_CPA_PKE_PUBLIC_KEY_SIZE: usize = v_T_AS_NTT_ENCODED_SIZE +. 32sz
+
+let v_CPA_PKE_CIPHERTEXT_SIZE: usize = v_VECTOR_U_ENCODED_SIZE +. v_VECTOR_V_ENCODED_SIZE
+
+let v_CPA_PKE_MESSAGE_SIZE: usize = 32sz
+
+// let v_CPA_SERIALIZED_KEY_LEN: usize =
+//   ((v_CPA_PKE_SECRET_KEY_SIZE +. v_CPA_PKE_PUBLIC_KEY_SIZE <: usize) +.
+//     Libcrux.Kem.Kyber768.Parameters.Hash_functions.v_H_DIGEST_SIZE
+//     <:
+//     usize) +.
+//   v_CPA_PKE_MESSAGE_SIZE
+  
