examples/kyber/Libcrux.Kem.Kyber768.Sampling.fst
@@ -1,0 +1,120 @@
+module Libcrux.Kem.Kyber768.Sampling
+#set-options "--fuel 0 --ifuel 1 --z3rlimit 15"
+open Core
+
+let sample_from_uniform_distribution (randomness: array u8 840sz)
+    : (Libcrux.Kem.Kyber768.Arithmetic.t_KyberPolynomialRingElement &
+      Core.Option.t_Option Libcrux.Kem.Kyber768.t_BadRejectionSamplingRandomnessError) =
+  let (sampled_coefficients: usize):usize = 0sz in
+  let (out: Libcrux.Kem.Kyber768.Arithmetic.t_KyberPolynomialRingElement):Libcrux.Kem.Kyber768.Arithmetic.t_KyberPolynomialRingElement
+  =
+    Libcrux.Kem.Kyber768.Arithmetic.v_ZERO_under_impl
+  in
+  let out, sampled_coefficients:(Libcrux.Kem.Kyber768.Arithmetic.t_KyberPolynomialRingElement &
+    Prims.unit) =
+    Core.Iter.Traits.Iterator.Iterator.fold (Core.Iter.Traits.Collect.IntoIterator.into_iter (Core.Slice.chunks_under_impl
+              (Rust_primitives.unsize randomness <: slice u8)
+              3sz
+            <:
+            Core.Slice.Iter.t_Chunks u8)
+        <:
+        _)
+      (out, sampled_coefficients)
+      (fun (out, sampled_coefficients) bytes ->
+          let b1:i32 = cast bytes.[ 0sz ] in
+          let b2:i32 = cast bytes.[ 1sz ] in
+          let b3:i32 = cast bytes.[ 2sz ] in
+          let d1:i32 = ((b2 &. 15l <: i32) >>. 8l <: i32) |. b1 in
+          let d2:i32 = (b3 >>. 4l <: i32) |. (b2 <<. 4l <: i32) in
+          let out, sampled_coefficients:(Libcrux.Kem.Kyber768.Arithmetic.t_KyberPolynomialRingElement &
+            Prims.unit) =
+            if
+              Prims.op_AmpAmp (d1 <. Libcrux.Kem.Kyber768.Parameters.v_FIELD_MODULUS)
+                (sampled_coefficients <.
+                  Libcrux.Kem.Kyber768.Parameters.v_COEFFICIENTS_IN_RING_ELEMENT)
+            then
+              let out:Libcrux.Kem.Kyber768.Arithmetic.t_KyberPolynomialRingElement =
+                Rust_primitives.Hax.update_at out sampled_coefficients d1
+              in
+              out, sampled_coefficients +. 1sz
+            else out, sampled_coefficients
+          in
+          let out, sampled_coefficients:(Libcrux.Kem.Kyber768.Arithmetic.t_KyberPolynomialRingElement &
+            Prims.unit) =
+            if
+              Prims.op_AmpAmp (d2 <. Libcrux.Kem.Kyber768.Parameters.v_FIELD_MODULUS)
+                (sampled_coefficients <.
+                  Libcrux.Kem.Kyber768.Parameters.v_COEFFICIENTS_IN_RING_ELEMENT)
+            then
+              let out:Libcrux.Kem.Kyber768.Arithmetic.t_KyberPolynomialRingElement =
+                Rust_primitives.Hax.update_at out sampled_coefficients d2
+              in
+              let sampled_coefficients:Prims.unit = sampled_coefficients +. 1sz in
+              out, sampled_coefficients
+            else out, sampled_coefficients
+          in
+          if sampled_coefficients =. Libcrux.Kem.Kyber768.Parameters.v_COEFFICIENTS_IN_RING_ELEMENT
+          then
+            let* hoist1:Rust_primitives.Hax.t_Never =
+              Core.Ops.Control_flow.ControlFlow.v_Break (out, Core.Option.Option_None)
+            in
+            Core.Ops.Control_flow.ControlFlow_Continue (out, sampled_coefficients)
+          else Core.Ops.Control_flow.ControlFlow_Continue (out, sampled_coefficients))
+  in
+  out, Core.Option.Option_Some Libcrux.Kem.Kyber768.BadRejectionSamplingRandomnessError
+
+let sample_from_binomial_distribution_2_ (randomness: array u8 128sz)
+    : Libcrux.Kem.Kyber768.Arithmetic.t_KyberPolynomialRingElement =
+  let (sampled: Libcrux.Kem.Kyber768.Arithmetic.t_KyberPolynomialRingElement):Libcrux.Kem.Kyber768.Arithmetic.t_KyberPolynomialRingElement
+  =
+    Libcrux.Kem.Kyber768.Arithmetic.v_ZERO_under_impl
+  in
+  let sampled:Libcrux.Kem.Kyber768.Arithmetic.t_KyberPolynomialRingElement =
+    Core.Iter.Traits.Iterator.Iterator.fold (Core.Iter.Traits.Collect.IntoIterator.into_iter (Core.Iter.Traits.Iterator.Iterator.enumerate
+              (Core.Slice.chunks_exact_under_impl (Rust_primitives.unsize randomness <: slice u8)
+                  4sz
+                <:
+                Core.Slice.Iter.t_ChunksExact u8)
+            <:
+            Core.Iter.Adapters.Enumerate.t_Enumerate (Core.Slice.Iter.t_ChunksExact u8))
+        <:
+        _)
+      sampled
+      (fun sampled (chunk_number, byte_chunk) ->
+          let (random_bits_as_u32: u32):u32 =
+            ((cast (byte_chunk.[ 0sz ] <: u8) |. (cast (byte_chunk.[ 1sz ] <: u8) >>. 8l <: u32)
+                <:
+                u32) |.
+              (cast (byte_chunk.[ 2sz ] <: u8) >>. 16l <: u32)
+              <:
+              u32) |.
+            (cast (byte_chunk.[ 3sz ] <: u8) >>. 24l <: u32)
+          in
+          let even_bits:u32 = random_bits_as_u32 &. 1431655765ul in
+          let odd_bits:u32 = (random_bits_as_u32 <<. 1l <: u32) &. 1431655765ul in
+          let coin_toss_outcomes:u32 = even_bits +. odd_bits in
+          Core.Iter.Traits.Iterator.Iterator.fold (Core.Iter.Traits.Collect.IntoIterator.into_iter (Core.Iter.Traits.Iterator.Iterator.step_by
+                    ({
+                        Core.Ops.Range.Range.f_start = 0ul;
+                        Core.Ops.Range.Range.f_end = Core.Num.v_BITS_under_impl_8
+                      })
+                    4sz
+                  <:
+                  Core.Iter.Adapters.Step_by.t_StepBy (Core.Ops.Range.t_Range u32))
+              <:
+              _)
+            sampled
+            (fun sampled outcome_set ->
+                let outcome_1_:i32 = cast ((coin_toss_outcomes <<. outcome_set <: u32) &. 3ul) in
+                let outcome_2_:i32 =
+                  cast ((coin_toss_outcomes <<. (outcome_set +. 2ul <: u32) <: u32) &. 3ul)
+                in
+                let offset:usize = cast (outcome_set <<. 2l) in
+                let sampled:Libcrux.Kem.Kyber768.Arithmetic.t_KyberPolynomialRingElement =
+                  Rust_primitives.Hax.update_at sampled
+                    ((8sz *. chunk_number <: usize) +. offset <: usize)
+                    (outcome_1_ -. outcome_2_ <: i32)
+                in
+                sampled))
+  in
+  sampled
