examples/kyber/Libcrux.Kem.Kyber768.fst
@@ -1,0 +1,235 @@
+module Libcrux.Kem.Kyber768
+#set-options "--fuel 0 --ifuel 1 --z3rlimit 15"
+open Core
+
+let v_SHARED_SECRET_SIZE: usize = Libcrux.Kem.Kyber768.Parameters.v_CPA_PKE_MESSAGE_SIZE
+
+let v_KEY_GENERATION_SEED_SIZE: usize =
+  Libcrux.Kem.Kyber768.Parameters.v_CPA_PKE_KEY_GENERATION_SEED_SIZE +. v_SHARED_SECRET_SIZE
+
+let v_PUBLIC_KEY_SIZE: usize = Libcrux.Kem.Kyber768.Parameters.v_CPA_PKE_PUBLIC_KEY_SIZE
+
+// let v_SECRET_KEY_SIZE: usize =
+//   ((Libcrux.Kem.Kyber768.Parameters.v_CPA_PKE_SECRET_KEY_SIZE +.
+//       Libcrux.Kem.Kyber768.Parameters.v_CPA_PKE_PUBLIC_KEY_SIZE
+//       <:
+//       usize) +.
+//     Libcrux.Kem.Kyber768.Parameters.Hash_functions.v_H_DIGEST_SIZE
+//     <:
+//     usize) +.
+//   v_SHARED_SECRET_SIZE
+
+let v_CIPHERTEXT_SIZE: usize = Libcrux.Kem.Kyber768.Parameters.v_CPA_PKE_CIPHERTEXT_SIZE
+
+let t_Kyber768PublicKey = array u8 1184sz
+
+let t_Kyber768PrivateKey = array u8 2400sz
+
+let t_Kyber768Ciphertext = array u8 1088sz
+
+let t_Kyber768SharedSecret = array u8 32sz
+
+type t_BadRejectionSamplingRandomnessError =
+  | BadRejectionSamplingRandomnessError : t_BadRejectionSamplingRandomnessError
+
+(*
+let generate_keypair (randomness: array u8 64sz)
+    : Core.Result.t_Result (array u8 1184sz & array u8 2400sz) t_BadRejectionSamplingRandomnessError =
+  let ind_cpa_keypair_randomness:slice u8 =
+    randomness.[ {
+        Core.Ops.Range.Range.f_start = 0sz;
+        Core.Ops.Range.Range.f_end
+        =
+        Libcrux.Kem.Kyber768.Parameters.v_CPA_PKE_KEY_GENERATION_SEED_SIZE
+      } ]
+  in
+  let implicit_rejection_value:slice u8 =
+    randomness.[ {
+        Core.Ops.Range.RangeFrom.f_start
+        =
+        Libcrux.Kem.Kyber768.Parameters.v_CPA_PKE_KEY_GENERATION_SEED_SIZE
+      } ]
+  in
+  let ind_cpa_key_pair, sampling_a_error:(Libcrux.Kem.Kyber768.Ind_cpa.t_KeyPair &
+    Core.Option.t_Option t_BadRejectionSamplingRandomnessError) =
+    Libcrux.Kem.Kyber768.Ind_cpa.generate_keypair ind_cpa_keypair_randomness
+  in
+  let secret_key_serialized:array u8 2400sz =
+    Libcrux.Kem.Kyber768.Ind_cpa.serialize_secret_key_under_impl ind_cpa_key_pair
+      implicit_rejection_value
+  in
+  match sampling_a_error with
+  | Core.Option.Option_Some error -> Core.Result.Result_Err error
+  | _ ->
+    Core.Result.Result_Ok
+    (Libcrux.Kem.Kyber768.Ind_cpa.pk_under_impl ind_cpa_key_pair, secret_key_serialized)
+
+let encapsulate (public_key: array u8 1184sz) (randomness: array u8 32sz)
+    : Core.Result.t_Result (array u8 1088sz & array u8 32sz) t_BadRejectionSamplingRandomnessError =
+  let randomness_hashed:array u8 32sz =
+    Libcrux.Kem.Kyber768.Parameters.Hash_functions.v_H (Rust_primitives.unsize randomness
+        <:
+        slice u8)
+  in
+  let (to_hash: array u8 64sz):array u8 64sz =
+    Libcrux.Kem.Kyber768.Conversions.into_padded_array (Rust_primitives.unsize randomness_hashed
+        <:
+        slice u8)
+  in
+  let to_hash:array u8 64sz =
+    Rust_primitives.Hax.update_at to_hash
+      ({
+          Core.Ops.Range.RangeFrom.f_start
+          =
+          Libcrux.Kem.Kyber768.Parameters.Hash_functions.v_H_DIGEST_SIZE
+        })
+      (Core.Slice.copy_from_slice_under_impl (Core.Ops.Index.IndexMut.index_mut to_hash
+              ({
+                  Core.Ops.Range.RangeFrom.f_start
+                  =
+                  Libcrux.Kem.Kyber768.Parameters.Hash_functions.v_H_DIGEST_SIZE
+                })
+            <:
+            slice u8)
+          (Rust_primitives.unsize (Libcrux.Kem.Kyber768.Parameters.Hash_functions.v_H (Rust_primitives.unsize
+                      public_key
+                    <:
+                    slice u8)
+                <:
+                array u8 32sz)
+            <:
+            slice u8)
+        <:
+        slice u8)
+  in
+  let hashed:array u8 64sz =
+    Libcrux.Kem.Kyber768.Parameters.Hash_functions.v_G (Rust_primitives.unsize to_hash <: slice u8)
+  in
+  let k_not, pseudorandomness:(slice u8 & slice u8) =
+    Core.Slice.split_at_under_impl (Rust_primitives.unsize hashed <: slice u8) 32sz
+  in
+  let ciphertext, sampling_a_error:(array u8 1088sz &
+    Core.Option.t_Option t_BadRejectionSamplingRandomnessError) =
+    Libcrux.Kem.Kyber768.Ind_cpa.encrypt (Rust_primitives.unsize public_key <: slice u8)
+      randomness_hashed
+      pseudorandomness
+  in
+  let (to_hash: array u8 64sz):array u8 64sz =
+    Libcrux.Kem.Kyber768.Conversions.into_padded_array k_not
+  in
+  let to_hash:array u8 64sz =
+    Rust_primitives.Hax.update_at to_hash
+      ({
+          Core.Ops.Range.RangeFrom.f_start
+          =
+          Libcrux.Kem.Kyber768.Parameters.Hash_functions.v_H_DIGEST_SIZE
+        })
+      (Core.Slice.copy_from_slice_under_impl (Core.Ops.Index.IndexMut.index_mut to_hash
+              ({
+                  Core.Ops.Range.RangeFrom.f_start
+                  =
+                  Libcrux.Kem.Kyber768.Parameters.Hash_functions.v_H_DIGEST_SIZE
+                })
+            <:
+            slice u8)
+          (Rust_primitives.unsize (Libcrux.Kem.Kyber768.Parameters.Hash_functions.v_H (Rust_primitives.unsize
+                      ciphertext
+                    <:
+                    slice u8)
+                <:
+                array u8 32sz)
+            <:
+            slice u8)
+        <:
+        slice u8)
+  in
+  let (shared_secret: array u8 32sz):array u8 32sz =
+    Libcrux.Kem.Kyber768.Parameters.Hash_functions.v_KDF (Rust_primitives.unsize to_hash <: slice u8
+      )
+  in
+  if Core.Option.is_some_under_impl sampling_a_error
+  then Core.Result.Result_Err (Core.Option.unwrap_under_impl sampling_a_error)
+  else Core.Result.Result_Ok (ciphertext, shared_secret)
+
+let decapsulate (secret_key: array u8 2400sz) (ciphertext: array u8 1088sz) : array u8 32sz =
+  let ind_cpa_secret_key, secret_key:(slice u8 & slice u8) =
+    Core.Slice.split_at_under_impl (Rust_primitives.unsize secret_key <: slice u8)
+      Libcrux.Kem.Kyber768.Parameters.v_CPA_PKE_SECRET_KEY_SIZE
+  in
+  let ind_cpa_public_key, secret_key:(slice u8 & slice u8) =
+    Core.Slice.split_at_under_impl secret_key
+      Libcrux.Kem.Kyber768.Parameters.v_CPA_PKE_PUBLIC_KEY_SIZE
+  in
+  let ind_cpa_public_key_hash, implicit_rejection_value:(slice u8 & slice u8) =
+    Core.Slice.split_at_under_impl secret_key
+      Libcrux.Kem.Kyber768.Parameters.Hash_functions.v_H_DIGEST_SIZE
+  in
+  let decrypted:array u8 32sz =
+    Libcrux.Kem.Kyber768.Ind_cpa.decrypt ind_cpa_secret_key ciphertext
+  in
+  let (to_hash: array u8 64sz):array u8 64sz =
+    Libcrux.Kem.Kyber768.Conversions.into_padded_array (Rust_primitives.unsize decrypted <: slice u8
+      )
+  in
+  let to_hash:array u8 64sz =
+    Rust_primitives.Hax.update_at to_hash
+      ({ Core.Ops.Range.RangeFrom.f_start = Libcrux.Kem.Kyber768.Parameters.v_CPA_PKE_MESSAGE_SIZE }
+      )
+      (Core.Slice.copy_from_slice_under_impl (Core.Ops.Index.IndexMut.index_mut to_hash
+              ({
+                  Core.Ops.Range.RangeFrom.f_start
+                  =
+                  Libcrux.Kem.Kyber768.Parameters.v_CPA_PKE_MESSAGE_SIZE
+                })
+            <:
+            slice u8)
+          ind_cpa_public_key_hash
+        <:
+        slice u8)
+  in
+  let hashed:array u8 64sz =
+    Libcrux.Kem.Kyber768.Parameters.Hash_functions.v_G (Rust_primitives.unsize to_hash <: slice u8)
+  in
+  let k_not, pseudorandomness:(slice u8 & slice u8) =
+    Core.Slice.split_at_under_impl (Rust_primitives.unsize hashed <: slice u8) 32sz
+  in
+  let expected_ciphertext, _:(array u8 1088sz &
+    Core.Option.t_Option t_BadRejectionSamplingRandomnessError) =
+    Libcrux.Kem.Kyber768.Ind_cpa.encrypt ind_cpa_public_key decrypted pseudorandomness
+  in
+  let selector:u8 =
+    Libcrux.Kem.Kyber768.Constant_time_ops.compare_ciphertexts_in_constant_time (Rust_primitives.unsize
+          ciphertext
+        <:
+        slice u8)
+      (Rust_primitives.unsize expected_ciphertext <: slice u8)
+  in
+  let to_hash:array u8 32sz =
+    Libcrux.Kem.Kyber768.Constant_time_ops.select_shared_secret_in_constant_time k_not
+      implicit_rejection_value
+      selector
+  in
+  let (to_hash: array u8 64sz):array u8 64sz =
+    Libcrux.Kem.Kyber768.Conversions.into_padded_array (Rust_primitives.unsize to_hash <: slice u8)
+  in
+  let to_hash:array u8 64sz =
+    Rust_primitives.Hax.update_at to_hash
+      ({ Core.Ops.Range.RangeFrom.f_start = v_SHARED_SECRET_SIZE })
+      (Core.Slice.copy_from_slice_under_impl (Core.Ops.Index.IndexMut.index_mut to_hash
+              ({ Core.Ops.Range.RangeFrom.f_start = v_SHARED_SECRET_SIZE })
+            <:
+            slice u8)
+          (Rust_primitives.unsize (Libcrux.Kem.Kyber768.Parameters.Hash_functions.v_H (Rust_primitives.unsize
+                      ciphertext
+                    <:
+                    slice u8)
+                <:
+                array u8 32sz)
+            <:
+            slice u8)
+        <:
+        slice u8)
+  in
+  Libcrux.Kem.Kyber768.Parameters.Hash_functions.v_KDF (Rust_primitives.unsize to_hash <: slice u8)
+  *)
+  
