examples/kyber/Libcrux.Kem.fst
@@ -1,0 +1,4 @@
+module Libcrux.Kem
+#set-options "--fuel 0 --ifuel 1 --z3rlimit 15"
+open Core
+
